I proved lookup_blocks and add_blocks.

matrix.v
@@ -62,13 +62,6 @@ unfold mat_build; rewrite ?vlookup_conv,
 ?vlookup_map, ?vlookup_vseq; done.
 Qed.
 
-Lemma lookup_vzip_with {X Y Z} (f : X -> Y -> Z) u v (i : fin n) :
-  (vzip_with f u v)@i = f (u@i) (v@i).
-Proof.
-induction i; inv_vec u; inv_vec v;
-cbn; intros; [done|apply IHi].
-Qed.
-
 Lemma vec_ext {X} (a b : vec X n) :
   (∀ i, a@i = b@i) -> a = b.
 Proof.
@@ -76,6 +69,50 @@ revert b; induction a; intros; inv_vec b; intros. done.
 assert (H0 := H 0%fin); cbn in H0; subst. f_equal; apply IHa; intros i.
 assert (HS := H (FS i)); cbn in HS; done.
 Qed.
+
+Section Vector_append.
+
+Lemma fin_to_nat_eq (i j : fin n) :
+  fin_to_nat i = fin_to_nat j -> i = j.
+Proof.
+revert j; induction i; cbn; intros; inv_fin j; intros; try done.
+cbn in H; apply eq_add_S, IHi in H; subst; done.
+Qed.
+
+Lemma fin_sum_sig (i : fin (m + n)) :
+  { i_m : fin m | i < m /\ @eq nat i i_m } +
+  { i_n : fin n | i ≥ m /\ Nat.add m i_n = i }.
+Proof.
+destruct (lt_dec i m) as [H|H]; [left|right].
+- exists (nat_to_fin H); split.
+  done. symmetry; apply fin_to_nat_to_fin.
+- apply Nat.nlt_ge in H.
+  assert (Hi := fin_to_nat_lt i).
+  assert (Hi' : i - m < n) by lia.
+  exists (nat_to_fin Hi'); split.
+  done. rewrite fin_to_nat_to_fin; lia.
+Qed.
+
+Definition fin_sum (i : fin (m + n)) :=
+  match fin_sum_sig i with
+  | inl (exist _ i' _) => inl i'
+  | inr (exist _ i' _) => inr i'
+  end.
+
+Lemma vlookup_vapp {X} (u : vec X m) (v : vec X n) (i : fin (m + n)) :
+  (u +++ v) !!! i = match fin_sum i with
+  | inl i' => u !!! i'
+  | inr i' => v !!! i'
+  end.
+Proof.
+unfold fin_sum; destruct (fin_sum_sig i) as [Hi|Hi]; destruct Hi as (i'&Hi&Hi').
+- induction u; cbn. lia. inv_fin i; inv_fin i'; cbn; intros; try done.
+  apply IHu. apply lt_S_n, Hi. apply eq_add_S, Hi'.
+- induction u; cbn in *. apply fin_to_nat_eq in Hi'; subst; done.
+  inv_fin i; cbn; intros. done. apply IHu; lia.
+Qed.
+
+End Vector_append.
 
 End Vector_lookups.
 
@@ -105,7 +142,7 @@ Global Instance : Add vec := vzip_with add.
 Global Instance : Zero vec := vreplicate n 0.
 
 Lemma lookup_add u v i : (u + v)@i = u@i + v@i.
-Proof. apply lookup_vzip_with. Qed.
+Proof. apply vlookup_zip_with. Qed.
 
 Lemma lookup_zero i : 0@i = 0.
 Proof. apply vlookup_replicate. Qed.
@@ -322,19 +359,7 @@ Definition blocks {k l m n}
   (c : mat l m) (d : mat l n) : mat (k + l) (m + n) :=
   vzip_with vapp a b +++ vzip_with vapp c d.
 
-Definition fin_sum {m n} : fin (m + n) -> fin m + fin n :=
-  fin_plus_inv _ inl inr.
-
-Lemma fin_sum_spec {m n} (i : fin (m + n)) :
-  match fin_sum i with
-  | inl j => i < m /\ @eq nat j i
-  | inr j => i ≥ m /\ Nat.add m j = i
-  end.
-Proof.
-Admitted.
-
-Lemma lookup_blocks {k l m n} a b c d
-  (i : fin (k + l)) (j : fin (m + n)) (Hi : i < k) (Hj : j < m) :
+Lemma lookup_blocks {k l m n} a b c d (i : fin (k + l)) (j : fin (m + n)) :
   (blocks a b c d)@i@j =
   match fin_sum i, fin_sum j with
   | inl i', inl j' => a@i'@j'
@@ -343,9 +368,9 @@ Lemma lookup_blocks {k l m n} a b c d
   | inr i', inr j' => d@i'@j'
   end.
 Proof.
-assert (Hi' := fin_sum_spec i); assert (Hj' := fin_sum_spec j);
-destruct (fin_sum i) as [i'|i'], (fin_sum j) as [j'|j'].
-Admitted.
+unfold blocks; rewrite ?vlookup_conv, vlookup_vapp; destruct (fin_sum i);
+rewrite vlookup_zip_with, vlookup_vapp; destruct (fin_sum j); done.
+Qed.
 
 Theorem add_blocks {k l m n}
   (a a' : mat k m) (b b' : mat k n)
@@ -353,7 +378,9 @@ Theorem add_blocks {k l m n}
   blocks a b c d + blocks a' b' c' d' ≡
   blocks (a + a') (b + b') (c + c') (d + d').
 Proof.
-Admitted.
+intros i j; rewrite ?lookup_add, ?lookup_blocks.
+destruct (fin_sum i), (fin_sum j); rewrite ?lookup_add; done.
+Qed.
 
 Theorem mul_blocks {k l m n}
   (a : mat k m) (b : mat k n)
